better wish-pred name: it's about the data, not the Verify func

new/proof/github_com/sanjit_bhat/pav/ktcore_proof/ktcore.v
@@ -2,7 +2,7 @@ From New.generatedproof.github_com.sanjit_bhat.pav Require Import ktcore.
 From New.proof.github_com.sanjit_bhat.pav Require Import prelude.
 
 From New.proof.github_com.sanjit_bhat.pav Require Import
-  cryptoffi cryptoutil.
+  cryptoffi cryptoutil merkle.
 
 From New.proof.github_com.sanjit_bhat.pav.ktcore_proof Require Import
   serde.
@@ -31,7 +31,7 @@ Definition Blame := gset BlameTys.
 Axiom Blame_IntoVal : IntoVal Blame.
 Global Existing Instance Blame_IntoVal.
 
-Definition wish_VerifyVrfSig pk vrfPk sig : iProp Σ :=
+Definition wish_VrfSig pk vrfPk sig : iProp Σ :=
   let obj := VrfSig.mk' (W8 VrfSigTag) vrfPk in
   let enc := VrfSig.pure_enc obj in
   "#His_sig" ∷ cryptoffi.is_sig pk enc sig ∗
@@ -49,7 +49,7 @@ Lemma wp_SignVrf ptr_sk pk P sl_vrfPk vrfPk :
   {{{
     sl_sig sig, RET #sl_sig;
     "Hsl_sig" ∷ sl_sig ↦* sig ∗
-    "#Hwish_vrfSig" ∷ wish_VerifyVrfSig pk vrfPk sig
+    "#Hwish_vrfSig" ∷ wish_VrfSig pk vrfPk sig
   }}}.
 Proof.
   simpl. wp_start as "@". wp_auto.
@@ -78,9 +78,9 @@ Lemma wp_VerifyVrfSig sl_pk pk sl_vrfPk vrfPk sl_sig sig :
     (err : bool), RET #err;
     "Hgenie" ∷
       match err with
-      | true => ¬ wish_VerifyVrfSig pk vrfPk sig
+      | true => ¬ wish_VrfSig pk vrfPk sig
       | false =>
-        "#Hwish_vrfSig" ∷ wish_VerifyVrfSig pk vrfPk sig
+        "#Hwish_vrfSig" ∷ wish_VrfSig pk vrfPk sig
       end
   }}}.
 Proof.
@@ -102,7 +102,7 @@ Proof.
   - by iFrame.
 Qed.
 
-Definition wish_VerifyLinkSig pk ep link sig : iProp Σ :=
+Definition wish_LinkSig pk ep link sig : iProp Σ :=
   let obj := LinkSig.mk' (W8 LinkSigTag) ep link in
   let enc := LinkSig.pure_enc obj in
   "#His_sig" ∷ cryptoffi.is_sig pk enc sig ∗
@@ -120,7 +120,7 @@ Lemma wp_SignLink ptr_sk pk P epoch sl_link link :
   {{{
     sl_sig sig, RET #sl_sig;
     "Hsl_sig" ∷ sl_sig ↦* sig ∗
-    "#Hwish_linkSig" ∷ wish_VerifyLinkSig pk epoch link sig
+    "#Hwish_linkSig" ∷ wish_LinkSig pk epoch link sig
   }}}.
 Proof.
   simpl. wp_start as "@". wp_auto.
@@ -149,9 +149,9 @@ Lemma wp_VerifyLinkSig sl_pk pk epoch sl_link link sl_sig sig :
     (err : bool), RET #err;
     "Hgenie" ∷
       match err with
-      | true => ¬ wish_VerifyLinkSig pk epoch link sig
+      | true => ¬ wish_LinkSig pk epoch link sig
       | false =>
-        "#Hwish_linkSig" ∷ wish_VerifyLinkSig pk epoch link sig
+        "#Hwish_linkSig" ∷ wish_LinkSig pk epoch link sig
       end
   }}}.
 Proof.
@@ -319,6 +319,26 @@ Proof.
   iApply "HΦ".
   iFrame "∗#".
 Qed.
+
+Definition wish_Memb pk uid ver dig memb : iProp Σ :=
+  ∃ label mapVal,
+  let enc_label := ktcore.MapLabel.pure_enc (ktcore.MapLabel.mk' uid ver) in
+  let enc_val := ktcore.CommitOpen.pure_enc memb.(ktcore.Memb.PkOpen) in
+  "#His_vrf_proof" ∷ cryptoffi.is_vrf_proof pk enc_label memb.(ktcore.Memb.LabelProof) ∗
+  "#His_vrf_out" ∷ cryptoffi.is_vrf_out pk enc_label label ∗
+  "#His_mapVal" ∷ cryptoffi.is_hash (Some enc_val) mapVal ∗
+  "#Hwish_memb" ∷ merkle.wish_VerifyMemb label mapVal memb.(ktcore.Memb.MerkleProof) dig.
+
+Definition wish_ListMemb pk uid (prefixLen : w64) dig hist : iProp Σ :=
+  ([∗ list] ver ↦ memb ∈ hist,
+    wish_Memb pk uid (uint.Z prefixLen + ver) dig memb).
+
+Definition wish_NonMemb pk uid ver dig nonMemb : iProp Σ :=
+  ∃ label,
+  let enc := ktcore.MapLabel.pure_enc (ktcore.MapLabel.mk' uid ver) in
+  "#His_vrf_proof" ∷ cryptoffi.is_vrf_proof pk enc nonMemb.(ktcore.NonMemb.LabelProof) ∗
+  "#His_vrf_out" ∷ cryptoffi.is_vrf_out pk enc label ∗
+  "#Hwish_nonMemb" ∷ merkle.wish_VerifyNonMemb label nonMemb.(ktcore.NonMemb.MerkleProof) dig.
 
 End proof.
 End ktcore.
